correctness of ext gcd

examples/modular_inversion/proofs/ext_gcd_optmized.ec
@@ -51,9 +51,8 @@ module OptExtGcd = {
     (v1,v2,v3) <- (v,(1-u), v);
     (t1,t2,t3) <- (0,-1,-v);
 
-    (t1,t2,t3) <@ ExtGCD.opt_simplify_ts(t1, t2, t3, u, v);
-    (v1, v2, v3) <- (v-t1, -u-t2, -t3);
-
+    (t1,t2,t3) <@ ExtGCD.opt_simplify_ts(t1, t2, v, u, v);
+    (v1, v2, v3) <- (v-t1, -u-t2, t3);
     (t1, t2, t3) <- (u1-v1, u2-v2, u3-v3);
 
     while (t3 <> 0){
@@ -63,7 +62,7 @@ module OptExtGcd = {
       }else{
         (v1, v2, v3) <- (v-t1, -u-t2, -t3);
       }
-      (t1, t2, t3) <- (u1-v1, u2-v2, u3 - v3);
+      (t1, t2, t3) <- (u1-v1, u2-v2, u3-v3);
 
      }
       return (u1, u2, u3);
@@ -76,9 +75,8 @@ module OptExtGcd = {
     (v1,v2,v3) <- (v,(1-u), v);
     (t1,t2,t3) <- (0,-1,v);
 
-    (t1,t2,t3) <@ ExtGCD.opt_simplify_ts(t1, t2, t3, u, v);
+    (t1,t2,t3) <@ ExtGCD.opt_simplify_ts(t1, t2, v, u, v);
     (v1, v2, v3) <- (v-t1, -u-t2, t3);
-
     (t1, t2, t3) <- (u1-v1, u2-v2, `|u3-v3|);
 
     while (t3 <> 0){
@@ -103,7 +101,7 @@ module OptExtGcd = {
       (v2,v3) <- (1-u, v);
       (t2,t3) <- (-1, v);
 
-      (t2,t3) <@ simplify_ts(t2, t3, u, v);
+      (t2,t3) <@ simplify_ts(t2, v, u, v);
       (v2, v3) <- (-u-t2, t3);
 
       (t2, t3) <- (u2-v2, `|u3-v3|);
@@ -122,13 +120,15 @@ module OptExtGcd = {
       return (u2, u3);
   }
 
+
     proc main5(u : int, v : int) = {
       var u2,u3,v2,v3,t2,t3;
-      (v2,v3) <- ((1-u), v);
+
       (u2,u3) <- (0, u);
+      (v2,v3) <- (1-u, v);
       (t2,t3) <- (-1, v);
 
-      (t2,t3) <@ simplify_ts(t2, t3, u, v);
+      (t2,t3) <@ simplify_ts(t2, v, u, v);
       (v2, v3) <- (-u-t2, t3);
 
       (t2, t3) <- (u2-v2, `|u3-v3|);
@@ -137,31 +137,70 @@ module OptExtGcd = {
         (t2,t3) <@ simplify_ts(t2, t3, u, v);
         if (v3 < u3){
           (u2, u3) <- (t2, t3);
-          (t2, t3) <- (u2-v2, `|u3 - v3|);          
         }else{
           (v2, v3) <- (-u-t2, t3);
-          (t2, t3) <- (u2-v2, `|u3 - v3|);          
         }
+
+        t2 <- u2 - v2;
+        if (v3 < u3){
+          t3 <- u3 - v3;
+        }else{
+          t3 <- v3 - u3;
+        }
+
        }
       return (u2, u3);
-  }
+  }  
+  
   
 }.
 
 
-lemma opt_4 : equiv[ OptExtGcd.main4 ~ OptExtGcd.main5 : ={arg} /\ 0 < u{1} /\ 0 < v{1}
-       ==>  ={res}].
-proc.
-wp. simplify.
-sp.
-while (={t2,t3,u2,u3,v2,v3,u,v}). wp.
-inline*. sp. wp. 
-while (={t20,t30,u0,v0}).
-wp. skip. progress. skip. progress. wp.
-inline*. sp. wp. 
-while (={t20,t30,u0,v0}).
-wp. skip. progress. skip. progress.
+lemma opt_0 : equiv[ ExtGCD.main2 ~ OptExtGcd.main1 : ={arg} /\ 0 < u{1} /\ 0 < v{1} ==> ={res} ].
+proc. sp. simplify.
+unroll {1} 1.
+rcondt {1} 1. progress. skip. smt().
+sim. 
 qed.
+
+
+lemma opt_1 : equiv[ OptExtGcd.main1 ~ OptExtGcd.main2  : ={arg} /\ 0 < u{1} /\ 0 < v{1} ==> ={res} ].
+proc.
+seq 3 3 : (={u,v,u1,u3,v1,v3,t1,u2,v2,t2,t3} /\ 0 < u{1} /\ 0 < v{1} /\ t3{1} < 0 /\ t3{1} = -v{1}).
+wp. skip. progress. smt. 
+seq 1 1 : (={u,v,u1,u3,v1,v3,t1,u2,v2,t2} /\ `|t3{1}| = t3{2}  /\ 0 < u{1} /\ 0 < v{1} /\ t3{1} < 0).    
+seq 1 1 : (={u,v,u1,u3,v1,v3,t1,u2,v2,t2} /\ `|t3{1}| = t3{2} /\ 0 < u{1} /\ 0 < v{1} /\ t3{1} < 0).
+ecall (gcd_t_simp_eq2 t3{1}). skip. progress. smt. smt.  
+skip. progress.
+rcondf {1} 1. progress. skip. smt.
+seq 2 2 : (={u,v,u1,u3,v1,v3,t1,u2,v2,t2,t3} /\ t3{1} = u3{1} - v3{1}).
+wp. skip. progress. smt. smt. 
+while (={u,v,u1,u3,v1,v3,t1,u2,v2,t2,t3} /\ t3{1} = u3{1} - v3{1}).
+wp. simplify.
+ecall (gcd_t_simp_eq3 t3{1}). skip. progress;smt.
+skip. progress.
+qed.    
+
+
+lemma opt_2 : equiv[ OptExtGcd.main2 ~ OptExtGcd.main3 : ={arg} /\ 0 < u{1} /\ 0 < v{1} ==> ={res} ].
+proc.
+seq 3 3 : (={u,v,u1,u3,v1,v3,t1,u2,v2,t2} /\ `|t3{1}| = t3{2} /\ 0 < u{1} /\ 0 < v{1} /\ t3{1} < 0).
+wp. simplify.  skip. progress. smt. smt.
+seq 1 1 : (={u,v,u1,u3,v1,v3,t1,u2,v2,t2} /\ t3{1} = t3{2} /\ 0 < u{1} /\ 0 < v{1} ).
+ecall (gcd_t_simp_eq3 v{1}). skip. progress.   
+seq 1 1 : (={u,v,u1,u3,v1,v3,t1,u2,v2,t2} /\ t3{1} = t3{2} /\ 0 < u{1} /\ 0 < v{1}).
+wp. skip. progress. 
+seq 1 1 : (={u,v,u1,u3,v1,v3,t1,u2,v2,t2} /\ `|t3{1}| = t3{2} /\ 0 < u{1} /\ 0 < v{1} /\ t3{1} = u3{1} - v3{1}).
+wp. skip. simplify.  progress.  
+while (={u,v,u1,u2,u3,v1,v2,v3,t1,t2} /\ t3{1} = u3{1} - v3{1} /\ `|t3{1}| = t3{2} /\ 0 < u{1} /\ 0 < v{1}).
+wp.
+exists* t3{1}. elim*. progress.
+call (gcd_t_simp_eq2 t3_L). simplify.
+skip. progress. 
+smt. smt. smt.  smt. smt. smt. smt. smt. smt. smt. smt. smt. smt. smt. 
+skip. progress. smt. smt.
+qed.
+
 
 
 lemma opt_3 : equiv[ OptExtGcd.main3 ~ OptExtGcd.main4 : ={arg} /\ 0 < u{1} /\ 0 < v{1}
@@ -178,28 +217,19 @@ wp. skip. progress. skip. progress.
 qed.
 
 
-lemma opt_2 : equiv[ OptExtGcd.main2 ~ OptExtGcd.main3 : ={arg} /\ 0 < u{1} /\ 0 < v{1} ==> ={res} ].
+lemma opt_4 : equiv[ OptExtGcd.main4 ~ OptExtGcd.main5 : ={arg} /\ 0 < u{1} /\ 0 < v{1}
+       ==>   ={res}].
 proc.
-seq 3 3 : (={u,v,u1,u3,v1,v3,t1,u2,v2,t2} /\ `|t3{1}| = t3{2} /\ 0 < u{1} /\ 0 < v{1} /\ t3{1} < 0).
-wp. simplify.  skip. progress. smt. smt.
-seq 1 1 : (={u,v,u1,u3,v1,v3,t1,u2,v2,t2} /\ `|t3{1}| = t3{2} /\ 0 < u{1} /\ 0 < v{1} /\ t3{1} < 0). admit.
-seq 1 1 : (={u,v,u1,u3,v1,v3,t1,u2,v2,t2} /\ `|t3{1}| = t3{2} /\ 0 < u{1} /\ 0 < v{1} /\ t3{1} < 0).
-wp. skip. progress. smt.
-seq 1 1 : (={u,v,u1,u3,v1,v3,t1,u2,v2,t2} /\ `|t3{1}| = t3{2} /\ 0 < u{1} /\ 0 < v{1} /\ t3{1} = u3{1} - v3{1}).
-wp. simplify.  progress.  
-while (={u,v,u1,u2,u3,v1,v2,v3,t1,t2} /\ t3{1} = u3{1} - v3{1} /\ `|t3{1}| = t3{2} /\ 0 < u{1} /\ 0 < v{1}).
-wp.
-exists* t3{1}. elim*. progress.
-call (gcd_t_simp_eq2 t3_L). simplify.
-skip. progress. 
-smt. smt. smt.  smt. smt. smt. smt. smt. smt. smt. smt. smt. smt. smt. 
-skip. progress. smt. smt.
+wp. simplify. sp.
+while (={t2,t3,u2,u3,v2,v3,u,v}). wp.
+inline*. sp. wp. 
+while (={t20,t30,u0,v0}).
+wp. skip. progress. skip. progress;smt.
+wp. inline*. sp. wp. 
+while (={t20,t30,u0,v0}).
+wp. skip. progress. skip. progress.
 qed.
 
 
-lemma opt_1 : equiv[ ExtGCD.main2 ~ OptExtGcd.main1 : ={arg} /\ 0 < u{1} /\ 0 < v{1} ==> ={res} ].
-proc. sp. simplify.
-unroll {1} 1.
-rcondt {1} 1. progress. skip. smt().
-sim. 
-qed.
+
+
